MLIR/Dialects/ArithSemantics.lean
@@ -178,8 +178,8 @@ private def add2: BasicBlockStmt arith := [mlir_bb_stmt|
 
 theorem add_commutative:
   forall (n m: FinInt 32),
-    run ⟦add1⟧ [[ ("n", ⟨.i32, n⟩), ("m", ⟨.i32, m⟩) ]] =
-    run ⟦add2⟧ [[ ("n", ⟨.i32, n⟩), ("m", ⟨.i32, m⟩) ]] := by
+    run ⟦add1⟧ (SSAEnv.One [ ("n", ⟨.i32, n⟩), ("m", ⟨.i32, m⟩) ]) =
+    run ⟦add2⟧ (SSAEnv.One [ ("n", ⟨.i32, n⟩), ("m", ⟨.i32, m⟩) ]) := by
   intros n m
   simp [Denote.denote]
   simp [run, add1, add2, denoteBBStmt, denoteOp]
